src/proof/dll_proof.v
@@ -20,9 +20,22 @@ Set Default Proof Using "W".
 #[global] Instance : IsPkgInit (iProp Σ) dll := define_is_pkg_init True%I.
 #[global] Instance : GetIsPkgInitWf (iProp Σ) dll := build_get_is_pkg_init_wf.
 
+(* l points to a dlist node whose prev pointer is p and the last next pointer is n *)
+Fixpoint is_dlist_node (l :  loc) (p : loc) (last : loc) (xs : list w64) : iProp Σ :=
+  match xs with
+  | [] => ⌜l = last⌝
+  | v :: xs =>
+    ∃ (n : loc),
+      "Hl" ∷ ⌜l ≠ null ⌝ ∗
+      "Hnext" ∷ l.[dll.Node.t, "next"] ↦ n ∗
+      "Hprev" ∷ l.[dll.Node.t, "prev"] ↦ p ∗
+      "His_dlist" ∷ is_dlist_node n l last xs
+  end.
+
 Definition own_list (l : loc) (xs : list w64) : iProp Σ :=
   ∃ (hd tl : loc),
     "Hhead" ∷ l.[dll.List.t, "head"] ↦ hd ∗
+    "His_dlist" ∷ is_dlist_node hd null null xs ∗
     "Htail" ∷ l.[dll.List.t, "tail"] ↦ tl ∗
     "Hsize" ∷ l.[dll.List.t, "size"] ↦ (W64 (length xs)).
 
@@ -33,7 +46,63 @@ Lemma wp_Len (l : loc) (xs : list w64) :
 Proof.
   wp_start as "Hown". iNamed "Hown".
   wp_auto.
-  iApply "HΦ". iFrame.
+  iApply "HΦ".
+  iFrame.
 Qed.
 
+Fixpoint Sorted (xs : list w64) :=
+  match xs with
+  | [] => True
+  | x :: xs => match xs with
+    | [] => True
+    | y :: _ => (uint.Z x < uint.Z y ∧ Sorted xs)
+    end
+  end.
+
+(* TODO: postcond should  intuitively denote xs = ys ++ y ++ z ++ zs and y < v < z with some side conditions for when they may be null*)
+Lemma t (l p last : loc) (v : w64) (xs : list w64):
+  {{{ is_pkg_init dll ∗ is_dlist_node l p last xs ∗ ⌜Sorted xs⌝ }}}
+    l @! (go.PointerType dll.Node) @! "findLeastGreaterNode" (# v)
+  {{{ prev node, RET #(prev, node); emp }}}.
+Proof.
+Abort.
+
+Theorem insertSorted_spec  (l : loc) (xs : list w64) (v : w64) :
+  {{{ is_pkg_init dll ∗ own_list l xs ∗ ⌜ Sorted xs ⌝  }}}
+    l @! (go.PointerType dll.List) @! "InsertSorted" #v
+  {{{ RET #(); ∃ ys zs, ⌜xs = ys ++ zs ⌝ ∗ ⌜Sorted (ys ++ v :: zs)⌝ ∗ own_list l (ys ++ v :: zs)}}}.
+Proof.
+  wp_start as "[Hown %HSorted]".
+  iNamed "Hown".
+  wp_auto.
+  wp_if_destruct.
+  - wp_alloc l' as "Hl".
+    wp_auto.
+    iApply "HΦ".
+    iAssert (⌜xs = []⌝)%I as "->".
+    { destruct xs as [|x xs]; [by done|].
+      simpl.
+      iDestruct "His_dlist" as "(%n & Hown)".
+      iNamedSuffix "Hown" "Node".
+      by iDestruct "HlNode" as "%HlNode".
+    }
+    iExists [], [].
+    iSplitR; [by done|].
+    iSplitR; [by done|].
+    rewrite /own_list.
+    iExists l', l'.
+    simpl.
+    iFrame.
+    iPoseProof (typed_pointsto_not_null l' {| dll.Node.val' := v; dll.Node.next' := null; dll.Node.prev' := null |} with "[$Hl]") as "%Hl".
+    iSplitL "".
+    + by iPureIntro.
+    + iStructNamed "Hl".
+      simpl.
+      iFrame.
+  -
+Admitted.
+
+Print is_dlist_node.
+
 End proof.
+
